Progress check on IMap; a case of using DSHCType for Calvin

coq/LLVMGen/Correctness_IMap2.v
@@ -50,6 +50,16 @@ Section DSHIMap_is_tfor.
     v'<- denoteIUnCType σ f vn v;;
     ret (mem_add offset v' acc).
 
+
+  (* | DSHIMap n x_p y_p f => *)
+  (*   '(x,i) <- resolve_PVar x_p ;; *)
+  (*   '(y,o) <- resolve_PVar y_p ;; *)
+  (*   loopcontblock <- incBlockNamed "IMap_lcont" ;; *)
+  (*   loopvar <- incLocalNamed "IMap_i" ;; *)
+  (*   '(body_entry, body_blocks) <- genIMapBody i o x y f loopvar loopcontblock ;; *)
+  (*   add_comment *)
+  (*     (genWhileLoop "IMap" (EXP_Integer 0%Z) (EXP_Integer (Z.of_nat n)) loopvar loopcontblock body_entry body_blocks [] nextblock) *)
+
   (* [tfor] formulation of [DSHIMap].
      "Reverse/downward" indexing ([n - 1 .. 0]). *)
   Definition DSHIMap_tfor_down
@@ -100,6 +110,346 @@ Section DSHIMap_is_tfor.
       cbn. assert (n - 0 - S i ≡ n - 1 - i) by lia. rewrite H0. reflexivity.
   Qed.
 
+  (* Lemma denoteDSHIMap_as_tfor: *)
+  (*   forall (σ : evalContext) n x y f, *)
+  (*     denoteDSHOperator σ (DSHIMap n x y f) ≈ DSHIMap_tfor_down σ f 0 n n x y. *)
+
+  Lemma eq_rev :
+    forall σ f n x y,
+      DSHIMap_tfor_up σ f 0 n x y ≈ DSHIMap_tfor_down σ f 0 n n x y.
+  Admitted.
+
+  Lemma DSHIMap_interpreted_as_tfor:
+    forall E σ (n : nat) (m : memoryH) f
+      (init acc : mem_block),
+      interp_helix (E := E) (denoteDSHIMap n f σ init acc) m ≈
+      tfor (fun k x' =>
+              match x' with
+              | None => Ret None
+              | Some (m', acc) => interp_helix (DSHIMap_body σ f k init acc) m'
+              end)
+        0 n (Some (m, acc)).
+  Proof.
+    intros.
+    rewrite denoteDSHIMap_as_tfor.
+    rewrite <- eq_rev.
+    unfold DSHIMap_tfor_up.
+    rewrite interp_helix_tfor; [|lia].
+    cbn.
+    apply eutt_tfor.
+    intros [[m' acc']|] i; [| reflexivity].
+    cbn.
+    repeat rewrite interp_helix_bind.
+    rewrite bind_bind.
+    apply eutt_eq_bind; intros [[?m ?] |]; [| rewrite bind_ret_l; reflexivity].
+    bind_ret_r2.
+    apply eutt_eq_bind.
+    intros [|]; reflexivity.
+  Qed.
+
+
+End DSHIMap_is_tfor.
+
+(* The result is a branch *)
+Definition branches (to : block_id) (mh : memoryH * ()) (c : config_cfg_T (block_id * block_id + uvalue)) : Prop :=
+  match c with
+  | (m,(l,(g,res))) => exists from, res ≡ inl (from, to)
+  end.
+
+Definition genIR_post (σ : evalContext) (s1 s2 : IRState) (to : block_id) (li : local_env)
+  : Rel_cfg_T unit ((block_id * block_id) + uvalue) :=
+  lift_Rel_cfg (state_invariant σ s2) ⩕
+               branches to ⩕
+               (fun sthf stvf => local_scope_modif s1 s2 li (fst (snd stvf))).
+
+Lemma DSHIMap_correct:
+  ∀ (n : nat) (x_p y_p : PExpr) (f : AExpr) (s1 s2 : IRState) (σ : evalContext) (memH : memoryH) 
+    (nextblock bid_in bid_from : block_id) (bks : list (LLVMAst.block typ)) (g : global_env) 
+    (ρ : local_env) (memV : memoryV),
+    genIR (DSHIMap n x_p y_p f) nextblock s1 ≡ inr (s2, (bid_in, bks))
+    → bid_bound s1 nextblock
+    → state_invariant σ s1 memH (memV, (ρ, g))
+    → Gamma_safe σ s1 s2
+    → no_failure (E := E_cfg) (interp_helix (denoteDSHOperator σ (DSHIMap n x_p y_p f)) memH)
+    → eutt (succ_cfg (genIR_post σ s1 s2 nextblock ρ))
+           (interp_helix (denoteDSHOperator σ (DSHIMap n x_p y_p f)) memH)
+            (interp_cfg (denote_ocfg (convert_typ [] bks) (bid_from, bid_in)) g ρ memV).
+Proof.
+  intros n x_p y_p f s1 s2 σ memH nextblock bid_in bid_from bks g ρ memV GEN NEXT PRE GAM NOFAIL.
+  Opaque genIMapBody.
+  Opaque genAExpr.
+  Opaque IntType.
+  Opaque incLocalNamed.
+  Opaque newLocalVar.
+
+  pose proof generates_wf_ocfg_bids _ NEXT GEN as WFOCFG.
+  pose proof inputs_bound_between _ _ _ GEN as INPUTS_BETWEEN.
+  pose proof genIR_Γ _ _ _ GEN as GENIR_Γ.
+  pose proof genIR_local_count _ _ _ GEN as GENIR_local.
+
+  (* Clean up PVars *)
+  cbn* in *; simp; cbn* in *.
+  hide_cfg.
+  inv_resolve_PVar Heqs1.
+  inv_resolve_PVar Heqs2.
+  unfold denotePExpr in *; cbn* in *.
+
+  simp; try_abs.
+
+  clean_goal.
+
+  repeat apply no_failure_Ret in NOFAIL.
+  edestruct @no_failure_helix_LU as (? & NOFAIL' & ?); eauto; []; clear NOFAIL; rename NOFAIL' into NOFAIL; cbn in NOFAIL; eauto.
+  edestruct @no_failure_helix_LU as (? & NOFAIL' & ?); eauto; []; clear NOFAIL; rename NOFAIL' into NOFAIL; cbn in NOFAIL; eauto.
+  clean_goal.
+
+  hred.
+  hstep; [eauto |].
+  hred; hstep; [eauto |].
+  hred.
+
+  (* We know that the Helix denotation can be expressed via the [tfor] operator *)
+  assert (NOFAIL_cont := NOFAIL).
+  apply no_failure_helix_bind_prefix in NOFAIL.
+
+  rewrite DSHIMap_interpreted_as_tfor.
+  rewrite DSHIMap_interpreted_as_tfor in NOFAIL.
+
+  match goal with
+  | [H : genWhileLoop ?prefix' _ _ ?loopvar' ?loopcontblock' ?body_entry' ?body_blocks' _ ?nextblock' ?s1' ≡ inr (?s2', (?entry_id', ?bks')) |- _] =>
+    remember prefix' as prefix
+      ; rename loopvar' into loopvar
+      ; rename loopcontblock' into loopcontblock
+      ; rename body_entry' into body_entry
+      ; rename body_blocks' into body_blocks
+      ; rename nextblock' into nextblock_
+      ; rename s1' into s1_
+      ; rename s2' into s2_
+      ; rename entry_id' into entry_id
+      ; rename bks' into bks
+  end.
+
+  cbn* in *; simp; cbn in *.
+
+  Transparent genIMapBody.
+  pose proof @genWhileLoop_tfor_correct prefix loopvar loopcontblock body_entry body_blocks nextblock_ entry_id s1_ s2_ i s1_ bks as GENC.
+  forward GENC; [clear GENC |].
+  {
+
+    clear -Heqs5.
+    rename Heqs5 into GEN.
+    Set Nested Proofs Allowed.
+
+    Lemma genWhileLoop_entry_in_scope_IMap:
+      ∀ (f : AExpr) (i0 : ident) (i1 : Int64.int) (i3 : ident) (i4 : Int64.int) (i6 : IRState) (loopcontblock : block_id) (loopvar : raw_id) 
+        (body_entry : block_id) (body_blocks : list (LLVMAst.block typ)) (s1_ : IRState),
+        genIMapBody i1 i4 i0 i3 f loopvar loopcontblock i6 ≡ inr (s1_, (body_entry, body_blocks)) → List.In body_entry (inputs body_blocks).
+    Proof.
+      induction f; intros *; try (cbn; intros GEN; clear -GEN; simp; cbn; auto; fail).
+    Qed.
+
+    eapply genWhileLoop_entry_in_scope_IMap; eauto.
+  }
+
+  forward GENC; [clear GENC |].
+  eauto. subst.
+  reflexivity.
+
+  forward GENC; [clear GENC |].
+  {
+    eauto using wf_ocfg_bid_add_comment.
+  }
+
+  forward GENC; [clear GENC |].
+  {
+    eapply lid_bound_between_shrink; [eapply lid_bound_between_newLocalVar | | ]; eauto; try reflexivity; solve_local_count.
+    subst.
+
+    destruct u.
+    eapply dropVars_local_count in Heqs7. rewrite Heqs7.
+    eapply genIMapBody_local_count in Heqs5. apply Heqs5.
+    (* TODO: solve_local_count doesn't work for dropVars properly? *)
+  }
+
+  forward GENC; [clear GENC |].
+  {
+    rewrite Forall_forall in INPUTS_BETWEEN. intros IN. subst.
+    inv VG.
+    rewrite inputs_convert_typ, add_comment_inputs in INPUTS_BETWEEN.
+    apply INPUTS_BETWEEN in IN; clear INPUTS_BETWEEN.
+    eapply not_bid_bound_between; eauto.
+  }
+
+  rename Heqs8 into WHILE.
+
+  specialize (GENC n WHILE).
+  match goal with
+    |- context[tfor ?bod _ _ _] => specialize (GENC _ bod)
+  end.
+
+  forward GENC; [clear GENC |].
+  {
+    clear -Heqs.
+    unfold MInt64asNT.from_nat in Heqs.
+    unfold MInt64asNT.from_Z in Heqs.
+    simp.
+    apply l0.
+  }
+
+  (* Invariant at each iteration *)
+  set (I := (fun (k : nat) (mH : option (memoryH * mem_block)) (stV : memoryV * (local_env * global_env)) =>
+               match mH with
+               | None => False
+               | Some (mH, b) => state_invariant σ s2_ mH stV
+               end)).
+  (* Precondition and postcondition *)
+  set (P := (fun (mH : option (memoryH * mem_block)) (stV : memoryV * (local_env * global_env)) =>
+               match mH with
+               | None => False
+               | Some (mH,b) => state_invariant σ s2_ mH stV
+               end)).
+
+  specialize (GENC I P P (Some (memH, x0))).
+
+
+  forward GENC; [clear GENC |].
+  {
+    subst I P; intros ? ? ? [[? []]|] * (INV & LOOPVAR & BOUNDk & RET); [| inv INV].
+
+    assert (EQk: MInt64asNT.from_nat k ≡ inr (Int64.repr (Z.of_nat k))).
+    {clear - BOUNDk Heqs.
+     destruct (MInt64asNT.from_nat k) eqn:EQ.
+     - exfalso.
+       unfold MInt64asNT.from_nat in *.
+       unfold MInt64asNT.from_Z in *.
+       simp; lia.
+     - unfold MInt64asNT.from_nat in *.
+       apply from_Z_intval in EQ.
+       rewrite EQ, repr_intval.
+       reflexivity.
+    }
+
+    rewrite EQk in *.
+    setoid_rewrite bind_ret_l.
+
+    eapply no_failure_tfor in NOFAIL. 3 : eauto. 2 : lia. cbn in NOFAIL.
+    rewrite interp_helix_bind in NOFAIL. rewrite EQk in NOFAIL.
+    assert (NOFAIL' := NOFAIL).
+    apply no_failure_bind_prefix in NOFAIL.
+
+    simp; try_abs. clear NOFAIL.
+    hvred.
+    eapply no_failure_bind_cont in NOFAIL'; cycle 1.
+    rewrite interp_helix_ret. constructor. cbn. reflexivity.
+    cbn in NOFAIL'.
+
+    Require Import Helix.LLVMGen.Correctness_AExpr.
+    pose proof @genAExpr_correct.
+    unfold denoteIUnCType.
+    clear RET.
+
+    Transparent genIMapBody. cbn in Heqs5. simp.
+    rename Heqs10 into AEXP.
+
+    match goal with
+    | [ |- context[denoteAExpr ?σ f]] => remember σ as aσ
+    end.
+
+
+    destruct u, u1.
+    eapply H1 in AEXP; clear H1; cycle 1.
+    - eapply state_invariant_enter_scope_DSHCType; cycle 1.
+      {
+        cbn.
+
+        clear WFOCFG INPUTS_BETWEEN NOFAIL'.
+        clear NOFAIL_cont H H0 NEXT LOOPVAR EQk BOUNDk Heqo1.
+        clear Heqs LUn EQsz LUn0 EQsz0 Heqo0 Heqo.
+
+        solve_gamma.
+      }
+
+      3 : eapply state_invariant_enter_scope_DSHnat; eauto.
+      3 : {
+        intros abs. eapply in_Gamma_Gamma_eq in abs; [| eapply incBlockNamed_Γ ; eauto].
+        eapply GAM; eauto.
+
+        eapply lid_bound_between_newLocalVar in Heqs4.
+        2:reflexivity.
+        eapply lid_bound_between_shrink; eauto.
+        solve_local_count.
+        apply dropVars_local_count in Heqs7.
+
+        apply genWhile_local_count in WHILE.
+        clear WFOCFG INPUTS_BETWEEN NOFAIL_cont NOFAIL'.
+        apply genAExpr_local_count in AEXP.
+        cbn in AEXP.
+        solve_local_count.
+      }
+      3 : {
+        clear WFOCFG INPUTS_BETWEEN NOFAIL'.
+        clear NOFAIL_cont H H0 NEXT LOOPVAR EQk BOUNDk Heqo1.
+        clear Heqs LUn EQsz LUn0 EQsz0 Heqo0 Heqo.
+
+        eapply state_invariant_Γ in GENIR_Γ; eauto.
+        solve_state_invariant.
+      }
+      3 : { reflexivity. }
+      solve_gamma.
+      solve_gamma.
+    - admit.
+    - admit.
+    - admit.
+    - admit.
+  }
+
+  forward GENC; [clear GENC |].
+  {
+    subst I P; cbn.
+    intros _ * BOUND INV; simp; auto.
+    (* TODO 1 *)
+    admit.
+  }
+
+  forward GENC; [clear GENC |].
+  {
+    admit.
+  }
+
+  forward GENC; [clear GENC |].
+  {
+    reflexivity.
+  }
+
+  forward GENC; [clear GENC |].
+  {
+    subst P I; red; intros; auto. 
+  }
+
+  forward GENC; [clear GENC |].
+  {
+    subst I P; red; intros; auto. 
+  }
+
+  specialize (GENC g ρ memV bid_from).
+  eapply eutt_mon.
+  {
+    clear GENC NOFAIL INPUTS_BETWEEN WFOCFG;subst P I.
+    intros [[? []] | ] (? & ? & ? & ?) *; cbn.
+    split; [| split]; cbn; eauto; admit.
+    - (* Need to enter scope,then escape it to link with s2 *)
+      (* eapply state_invariant_Γ; eauto; admit. *)
+      admit.
+  }
+  { subst P; cbn.
+    clear -PRE.
+    solve_state_invariant.
+    admit.
+  }
+Admitted.
+
+Section Swap.
+
   Definition pair_rel {A B} (RA : A -> A -> Prop) (RB : B -> B -> Prop) :=
     (fun '(a, b) '(a', b') => RA a a' /\ RB b b').
 
@@ -135,15 +485,10 @@ Section DSHIMap_is_tfor.
   Definition equiv_mem_block (n : nat) (m m' : mem_block) :=
     equiv_mem_block_frag 0 n m m'.
 
-  Notation "m ≡[ i , n  ] m'" := (equiv_mem_block_frag i n m m') (at level 10).
-  Notation "m ≡[ n ] m'" := (equiv_mem_block n m m') (at level 10).
-
-
   Instance option_pair_Equivalence: (Equivalence (⤉ (@eq memoryH, @equiv mem_block _))).
   Proof.
     intros. apply (@option_pair_rel_Equiv memoryH mem_block eq equiv _ mem_block_Equiv_Equivalence).
   Qed.
-
 
   Lemma imap_body_post:
     forall E m1 m2 init σ f i,
@@ -206,7 +551,7 @@ Section DSHIMap_is_tfor.
         → S i < n
         -> no_failure (E := void1) (interp_helix (vec <- tfor (λ (i0 : nat) (acc : mem_block), DSHIMap_body σ f i0 init acc) 0 (S i) init;;
                                 tfor (λ (i0 : nat) (acc : mem_block), DSHIMap_body σ f (n - 1 - i0) init acc) 0 (n - S i) vec) memH)
-        → eutt (E := void1) (⤉ (eq, equiv))
+        → eutt (E := void1) (⤉ (eq, equiv_mem_block n))
           (interp_helix (vec <- tfor (λ (i0 : nat) (acc : mem_block), DSHIMap_body σ f i0 init acc) 0 (S i) init;;
           tfor (λ (i0 : nat) (acc : mem_block), DSHIMap_body σ f (n - 1 - i0) init acc) 0 (n - S i) vec) memH)
           (interp_helix (vec <- tfor (λ (i0 : nat) (acc : mem_block), DSHIMap_body σ f (S (S i) - 1 - i0) init acc) 0 (S i) init;;
@@ -220,7 +565,7 @@ Section DSHIMap_is_tfor.
 
       assert (
         SWAP_LHS:
-          eutt (E := void1) (⤉ (eq, equiv))
+          eutt (E := void1) (⤉ (eq, equiv_mem_block n))
 
             (interp_helix (vec <- (tfor (λ (i0 : nat) (acc : mem_block), DSHIMap_body σ f i0 init acc) 0 i init) ;;
                            vec <- (tfor (λ (i0 : nat) (acc : mem_block), DSHIMap_body σ f i0 init acc) i (S i) vec) ;;
@@ -232,7 +577,7 @@ Section DSHIMap_is_tfor.
         eapply eutt_clo_bind. reflexivity.
 
         intros [[] |] [[]|] EQ; inv EQ.
-        2 : reflexivity.
+        2 : { apply eqit_Ret; constructor. }
         setoid_rewrite tfor_split with (j := n - S i) at 2; try lia.
         cbn.
 
@@ -277,6 +622,31 @@ Section DSHIMap_is_tfor.
         rewrite H0. clear H0 HeqRHS H RHS.
 
         setoid_rewrite interp_helix_bind.
+        eapply eqit_mon; auto.
+
+        Unshelve.
+        3 : exact (⤉ (eq, (fun x y => equiv_mem_block_frag i (S i) x y /\ equiv_mem_block_frag (S i) n x y))).
+        {
+          intros [[] |] [[] |] EQ; inv EQ. inv H1.
+          2 : constructor.
+          constructor. cbn. split; auto.
+          destruct H0.
+          Set Nested Proofs Allowed.
+
+          Lemma equiv_mem_block_split:
+            forall i j k m m',
+              i <= j -> S j <= k ->
+              equiv_mem_block_frag i (S j) m m' /\ equiv_mem_block_frag (S j) k m m' ->
+              equiv_mem_block k m m'.
+          Proof.
+            unfold equiv_mem_block, equiv_mem_block_frag; intros * B B' []. intros.
+
+            destruct (k0 <=? S j) eqn: EQ.
+            apply H. rewrite Nat.leb_le in EQ.
+          Admitted.
+          admit.
+        }
+
 
         (* match goal with *)
         (* | [ |- eutt _ (ITree.bind ?pre ?post) (ITree.bind ?pre' ?post') ] => *)
@@ -295,53 +665,48 @@ Section DSHIMap_is_tfor.
         (*   intros [[] |] EQ. subst. *)
         (*   destruct a as [[] |]. *)
 
-
-
         (*   intros. *)
         (* - admit. *)
         (* - admit. *)
-        admit.
-      }
 
-      setoid_rewrite bind_bind.
-      rewrite SWAP_LHS; clear SWAP_LHS.
-      rewrite IHi; try lia. clear IHi.
+      (* setoid_rewrite bind_bind. *)
+      (* rewrite SWAP_LHS; clear SWAP_LHS. *)
+      (* rewrite IHi; try lia. clear IHi. *)
 
-      assert (EQ : S i - 1 ≡ i) by lia; rewrite EQ; clear EQ.
-      setoid_rewrite tfor_unroll at 2.
+      (* assert (EQ : S i - 1 ≡ i) by lia; rewrite EQ; clear EQ. *)
+      (* setoid_rewrite tfor_unroll at 2. *)
 
-      assert (EQ : S i - 0 ≡ S i) by lia; rewrite EQ; clear EQ.
+      (* assert (EQ : S i - 0 ≡ S i) by lia; rewrite EQ; clear EQ. *)
 
-      assert (
-        SWAP_LHS:
-          eutt (E := void1) eq
-               (interp_helix
-                  (vec <- DSHIMap_body σ f (S i) init init;;
-                    tfor (λ (i0 : nat) (acc : mem_block), DSHIMap_body σ f (S i - i0) init acc) 1 (S i) vec ) memH)
-               (interp_helix
-                    (vec <- tfor (λ (i0 : nat) (acc : mem_block), DSHIMap_body σ f (S i - i0) init acc) 1 (S i) init ;;
-                     DSHIMap_body σ f (S i) init vec) memH)). {
-        setoid_rewrite interp_helix_bind.
-        eapply commut_gen; admit.
-      }
-      all : try lia.
+      (* assert ( *)
+      (*   SWAP_LHS: *)
+      (*     eutt (E := void1) eq *)
+      (*          (interp_helix *)
+      (*             (vec <- DSHIMap_body σ f (S i) init init;; *)
+      (*               tfor (λ (i0 : nat) (acc : mem_block), DSHIMap_body σ f (S i - i0) init acc) 1 (S i) vec ) memH) *)
+      (*          (interp_helix *)
+      (*               (vec <- tfor (λ (i0 : nat) (acc : mem_block), DSHIMap_body σ f (S i - i0) init acc) 1 (S i) init ;; *)
+      (*                DSHIMap_body σ f (S i) init vec) memH)). { *)
+      (*   setoid_rewrite interp_helix_bind. *)
+      (*   eapply commut_gen; admit. *)
+      (* } *)
+      (* all : try lia. *)
 
-      setoid_rewrite interp_helix_bind at 2.
-      rewrite SWAP_LHS; clear SWAP_LHS.
-      rewrite <- interp_helix_bind.
-      rewrite tfor_ss_dep.
-      all : try lia.
-      2 : { Unshelve. 4 : exact (fun n mem_bl => DSHIMap_body σ f (i - n) init mem_bl). intros; reflexivity. shelve. shelve. }
-      setoid_rewrite bind_bind.
-      setoid_rewrite interp_helix_bind.
-      eapply eutt_clo_bind. reflexivity.
+      (* setoid_rewrite interp_helix_bind at 2. *)
+      (* rewrite SWAP_LHS; clear SWAP_LHS. *)
+      (* rewrite <- interp_helix_bind. *)
+      (* rewrite tfor_ss_dep. *)
+      (* all : try lia. *)
+      (* 2 : { Unshelve. 4 : exact (fun n mem_bl => DSHIMap_body σ f (i - n) init mem_bl). intros; reflexivity. shelve. shelve. } *)
+      (* setoid_rewrite bind_bind. *)
+      (* setoid_rewrite interp_helix_bind. *)
+      (* eapply eutt_clo_bind. reflexivity. *)
 
-      intros [[] |] [[] |] EQ; inv EQ. 2 : reflexivity.
-      rewrite tfor_split with (j := (S (S i))); try lia.
-      rewrite tfor_unroll. setoid_rewrite tfor_0.
-      rewrite bind_ret_r. reflexivity. lia.
-      Unshelve.
+      (* intros [[] |] [[] |] EQ; inv EQ. 2 : reflexivity. *)
+      (* rewrite tfor_split with (j := (S (S i))); try lia. *)
+      (* rewrite tfor_unroll. setoid_rewrite tfor_0. *)
+      (* rewrite bind_ret_r. reflexivity. lia. *)
+      (* Unshelve. *)
 
   Admitted.
-
-End DSHIMap_is_tfor.
+End Swap.
